---
title: DS Lecture 14
author: Shashwat Singh
code: ma5.101
number: 14
---


## Functions
#### Definition:
A binary function is defined by two sets say $X$ and $Y$
A binary relation $f$ from $X \rightarrow Y$  is called a function if *each* element in $X$ maps to exactly one element in $Y$.  
Do note: every element in $X$ *has* to be mapped to an element.
- The set $X$ is the *domain* and the set $Y$ is the *co-domain*
- The image of $y \in Y$ of an element $x \in X$ is denoted by $y = f(x)$
- For aa function $f: X\rightarrow Y$ , if $y\in Y$ then the pre-image of $y$ is an element $x\in X$ for which $f(x) = y$
- The set of all elemenets in $Y$ which have atleast one pre-image is called the image of $f$ and is denoted by $Im(f)$

### Partial Functions
A partial function $f: X \rightarrow Y$ is defined every element $x \in D$ ($D \subset X$) maps to *one* element in $Y$.  
Do note that strictly speaking a Partial function is *not* a function.

## Type of functions 
#### One-to-one or injective function
- A function $f: X \rightarrow Y$ is 1-1 or *injective* if each element in co-domain is the image of *at most* one element in the the domain. 
- In other words, $f: X \rightarrow Y$ is 1-1 if $a, b \in X$ such that $a \not= b \implies f(a) \not=f(b)$  
- contrapositive (and therefore implied): $f(a) = f(b) \implies a = b$ 
- If a function is note one-to-one it is called **many-one**.

#### Onto function or surjective
- for $f: X \rightarrow Y$ , if each element of co-domain Y is the image of *atleast one* element in in $X$ 
- In other words $f: X \rightarrow Y$ is onto iff $Im(f) = Y$.

#### Bijective or one-one correspondence
- If a function is both *injective* and *surjective*

**Theorem**: If a function $f: X \rightarrow Y$ is *injective*, then $f: X \rightarrow Im(f)$ is a *bijection*.  
    **Proof**: The definition of *surjection* implies that the co-domain of a surjective function is equal to $Im(f)$.
                      Thus $f: X \rightarrow Im(f)$ is *surjective* (i).
                      Given that $f: X \rightarrow Y$ is *injective* $\implies$ every element $y \in Y$ has at most one pre-image. 
                      $z \in Im(f) \implies z \in Y, \forall z \in Im(f)$ as $Im(f)\subseteq Y$ thus every element in $Im(f)$ has at most one pre-image in $X$
                       this $f: X \rightarrow Im(f)$ is also injective (ii)
                       By (i) and (ii) the function is *bijective*

  **Theorem**: If a function $f: X \rightarrow Y$ is *injective*, and $X, Y$ are finite sets of the same size then $f: X \rightarrow Y$ is a bijection.
                
   Let $f: X \rightarrow Y$ is a function with $|X| = m, |Y| = n$ then: 
   - Total number of functions from $X \rightarrow Y$ is $n^m$ 
        reasoning: every element in $X$ *needs* to have an image in $Y$ and thus has $n$ choices thus $n^m$
   - The total number of injective functions $X \rightarrow Y$ with $m \leq n$ is ${n \choose m} m!$ . 
        reasoning: we choose m eleents in $Y$ and then all possible rearrangements of these will yield the total number of mappings.
   - The total number of surjective functions from $X \rightarrow Y$ with $m \geq n$ is $n! S(m, n)$ where S refers to the Stirling number of second kind
        resoning: Stirling number of second kind gives you the number of ways to partition a particular set of $m$ elements into $n$ non-empty sets. Thus what we're doing is partitioning the $X$ into $n$ subsets, and then we can associate each sub-set with an element of $Y$ (a subset for each element). For each partition there are $n!$ possible mappings. 
   - Total number of bijective functions from $X \rightarrow Y$ with $m = n$ is $n!$ 

### Inverse functions
A function is *bijective* $f: X \rightarrow Y$ then we define $g: Y \rightarrow X$ such that $g(y) = x \forall y \in Y, x\in X$ 
The $g$ is the inverse of $f$ 
### One-way function
A function $f: X \rightarrow Y$ is called a one-way function if $f(x)$ is easy to compute $\forall x \in X$ but it is *generally* infeasible to compute 
$x \in X | f(x) = y, y \in Y$ 
Note: emphasis has been given to "generally" because there may be some values $y \in Y$ for which is it is easy to find $x \in X$ such that $y = f(x)$ 
Such a function may or may not be bijective.
### Trap-door one-way function 
Iti s a *one-way* function $f: X \rightarrow Y$ with the additional property that given some extra information it becomes feasible to get $x \in X$ such that $f(x) = y, y \in Im(f)$ 

### Involutions
**Definition**: let $f$ be a bijection on a set $S$ this $f: S \rightarrow S$ then the function $f$ is set to be an involution iff $f = f^-1$ or equivalently 
$f(f(x)) = x$  


### Composition of function
**Definition**: Let $f: A \rightarrow B$ and $g: B \rightarrow C$ be two functions. The composition of $f$ by $g$ be the function $(g \circ f)(a) = g[f(a)] \forall a \in A$  
$g \circ f: A \rightarrow C$  
Such a composition can also be described for $f: A \rightarrow B$ , $g: C \rightarrow D$ if $C \subseteq B$  
**Lemma**: Let $f: A \rightarrow B$ , $g: B \rightarrow C$ and $h: C \rightarrow D$ then whenever the compositions involved are defined we can say:
$$
(f \circ g) \circ h = f \circ (g \circ h)
$$
*associacitivity*

### Identity function
The identity function $I_s: S \rightarrow S$ such that $I_s(x) = x \forall x \in S$ . This can also be represented by $1_s$  
**Theorem**: Let $f: S \rightarrow T$ and $1_s$ and $1_t$ then:
$$
(f \circ 1_s) = (1_t \circ f) = f
$$  

**Proof**:  
Given:  
$$
1_s: S \rightarrow S | 1_S(s) = s \forall s \in S \\
1_t: T \rightarrow T | 1_T(t) = t \forall t \in T  \\
\text{Therefore}, \\
(f \circ 1_S): S \rightarrow T\\
(f \circ 1_S)(s) = f(1_S(s)) = f(s) \forall s \in S [\textrm{By definition of } 1_s] \\
Similarly, \\
(1_T \circ f): S \rightarrow T \\
(1_T \circ f)(t) = i_T(f(s)) = f(s) \forall s \in S [\textrm{By definition of } 1_t] \\
\textrm{thus, }\\
(f \circ 1_S) = (1_T \circ f) = f
$$

### Characteristic function
Any set $S|S \subseteq U$ can be associated with a *characteristic function* $e_S$ such that
$$
e_S: U \rightarrow {0, 1} \\
e_s(x) = 
\begin{array}{cc}
    \Bigg\{ & \begin{array}{cc}
        1 & x \in S \\
        0 & x \notin S
     \end{array}
 \end{array}
$$

### Inverses of functions
Let $f: S \rightarrow T$ and $g: T \rightarrow S$  be two mappings. 
if $g \circ f = 1_S$ then $g$ is the left inverse of $f$
if $f \circ g = 1_T$ then $g$ is the right inverse of $f$ 

A function which has a two-sided inverse is called *invertible*
**Theorem**: 
- A function is left invertible iff it is injective.
- A function is right invertible iff it is surjective.
- And thus a function is invertible iff it is bijective
**Corollary**
- A function $f: A \rightarrow B$ is *bijective* iff it has both: a left inverse and a right inverse.
**Corollary**
- If $g \circ f$ is defined, and both f and g have left inverse then $g \circ f$ has a left inverse.

**Doubt: can a bijective function have a left inverse which is different from it's right inverse?**


### Idempotent functions
Let for all $f: S \rightarrow S$  $f^2 = f \circ f$ 
if $f^2 = f$ then $f$ is said to be idempotent or a projection.



**Theorems:**  
For the following function definitions: \\
$$
f: A \rightarrow B \\
g: B \rightarrow C \\
g \circ f: A \rightarrow c
$$

1. If $f$ and $g$ are both injective then $g \circ f$ and  are injective as well
2. If $f$ and $g$ are both surjective then $g \circ f$ and  are surjective as well.
3. and therefore if $f$ and $g$ are bijective then so are $f \circ g$ and $g \circ f$ 
4. and also $(f \circ g)^{-1} = f^{-1} \circ g^{-1}$ 
5. if $g \circ f$ is injective, $f$ is injective
6. if $g \circ f$ is surjective, $g$ is surjective too. 

**Proofs**  
$$
\text{for all proofs that are to follow: } \\
f: A \rightarrow B \\
g: B \rightarrow C \\
\text{thus} \\
g \circ f: A \rightarrow C
$$

for (1.)
$$
\text{Given } f \text{ and } g \text{ are both injective} \\
f(x_1) = f(x_2) \implies x_1 = x_2, \text{ for arbitrary } x_1 \text{ and } x_2 \\
g(x_1) = g(x_2) \implies x_1 = x_2, \text{ for arbitrary } x_1 \text{ and } x_2 \\
\text{let}
g \circ f (x_1) = g \circ f(x_2) \\
\implies g(f(x_1)) = g(f(x_2)) \\
\implies g(x_1) = g(x_2) \text{ as f is injective } \\
\implies x_1 = x_2 \text{ as g is injective} \\
$$




**Theorem**: If $X$ and $Y$ are two non-empty sets and $f$ is a mapping of $X$ into $Y$. Then, for any sub-sets $A, B \subseteq X$ 
then: $f(A \cup B) = f(A) \cup f(B)$ 
**Proof**
RTP:
1. $f(A \cup B) \subseteq f(A) \cup f(B)$
2. $f(A) \cup f(B) \subseteq f(A \cup B)$ 

Let $y$ be an arbitrary element such that $y \in f(A \cup B)$
<div>
$$
y \in f(A \cup B) \\
\begin{align}
	& \implies y = f(x), \exists x \in (A \cup B) \text{ by definition of the function} \\
	& \implies y = f(x), \exists x \in A \lor x \in B \\
	& \implies y \in f(A) \lor y \in f(B) \\
	& \implies y \in f(A) \cup f(B) \\
\end{align}
$$
</div>

$\text{thus proved } f(A \cup B) \subseteq f(A) \cup f(B).....(\text{i})$

$\text{Let } y \in f(A) \cup f(B) \text{ be an arbitrary variable}$

<div>
$$
\begin{align}
	\implies y \in f(A) \cup f(B) \\
	\implies y \in f(A) \lor y \in f(B) \\
	\implies y = f(x), \exists x \in A \lor x \in B \\
	\implies y = f(X), \exists x \in A \cup B \\
	\implies y \in f(A \cup B)
\end{align}
$$
</div>

Thus,
$f(A) \cup f(B) \subseteq f(A \cup B)........(\text{ii})$

$\text{ by i and ii, } f(A) \cup f(B) = f(A \cup B)$


**Theorem**  
If $X$ and $Y$ are two non-empty sets and $f$ be a bijective function such that $f: X \rightarrow Y$ 
then for $A, B \subseteq Y$
$f^{-1}(A \cup B) = f^{-1}(A) \cup f^{-1}(B)$

**Theorem**  
if $f: X \rightarrow Y$ be a mapping anf $A, B \subseteq X$ then $f(A \cap B) \subseteq f(A) \cup f(B)$  
Note: *The equality holds in the case of $f$ being a bijection*
